lib/Buckets/PackedKV.i.dfy
@@ -1,6 +1,7 @@
 include "PackedStringArray.i.dfy"
 include "../Base/total_order.i.dfy"
 include "KVList.i.dfy"
+include "../Base/NativeArrays.s.dfy"
 
 module PackedKV {
   import PackedStringArray
@@ -12,7 +13,9 @@ module PackedKV {
   import opened ValueMessage
   import opened BucketsLib
   import opened Options
-
+  import opened NativeArrays
+  import Uint32_Order
+  
   datatype Pkv = Pkv(
       keys: PackedStringArray.Psa,
       messages: PackedStringArray.Psa)
@@ -291,5 +294,37 @@ module PackedKV {
       i := i + 1;
     }
     return true;
+  }
+
+  method MergePart(oldpkv: Pkv, newpkv: Pkv, start: uint64, end: uint64)
+    returns (resultpkv: Pkv, newstart: uint64)
+    requires WF(oldpkv)
+    requires WF(newpkv)
+    requires start as int <= end as int < |newpkv.keys.offsets|
+  {
+    PackedStringArray.psaStartsLte(newpkv.keys, start, end);
+    var maxkeyslen :=
+      |oldpkv.keys.data| as uint64
+      + PackedStringArray.psaStart(newpkv.keys, end) as uint64
+      - PackedStringArray.psaStart(newpkv.keys, start) as uint64;
+    var maxkeysoffsetslen := |oldpkv.keys.offsets| as uint64 + end - start;
+    var newkeys := newArrayFill(maxkeyslen, 0);
+    var newkeyoffsets := newArrayFill(maxkeysoffsetslen, 0);
+
+    PackedStringArray.psaStartsLte(newpkv.messages, start, end);
+    var maxmessageslen :=
+      |oldpkv.messages.data| as uint64
+      + PackedStringArray.psaStart(newpkv.messages, end) as uint64
+      - PackedStringArray.psaStart(newpkv.messages, start) as uint64;
+    var maxmessagesoffsetslen := |oldpkv.messages.offsets| as uint64 + end - start;
+    var newmessages := newArrayFill(maxmessageslen, 0);
+    var newmessagesoffsets := newArrayFill(maxmessagesoffsetslen, 0);
+
+    var oldindex := 0;
+    var newindex := start;
+    while oldindex < |oldpkv.keys.offsets| && newindex < end
+    {
+    }
+    
   }
 }
